Source/Dafny/Compilers/Compiler-python.cs
@@ -106,6 +106,15 @@ namespace Microsoft.Dafny {
         return Compiler.CreateMethod(m, typeArgs, createBody, MethodWriter, forBodyInheritance, lookasideBody);
       }
 
+      public ConcreteSyntaxTree CreateFreshMethod(Method m) {
+        throw new NotImplementedException();
+      }
+
+      public ConcreteSyntaxTree CreateMockMethod(Method m, List<TypeArgumentInstantiation> typeArgs, bool createBody, bool forBodyInheritance,
+        bool lookasideBody) {
+        throw new NotImplementedException();
+      }
+
       public ConcreteSyntaxTree CreateFunction(string name, List<TypeArgumentInstantiation> typeArgs,
         List<Formal> formals, Type resultType, IToken tok, bool isStatic,
         bool createBody, MemberDecl member, bool forBodyInheritance, bool lookasideBody) {
