Source/Dafny/Compilers/Compiler.cs
@@ -93,7 +93,8 @@ namespace Microsoft.Dafny {
     protected abstract string GetHelperModuleName();
     protected interface IClassWriter {
       ConcreteSyntaxTree/*?*/ CreateMethod(Method m, List<TypeArgumentInstantiation> typeArgs, bool createBody, bool forBodyInheritance, bool lookasideBody);
-      ConcreteSyntaxTree/*?*/ CreateMockMethod(Method m);
+      ConcreteSyntaxTree/*?*/ CreateFreshMethod(Method m);
+      ConcreteSyntaxTree/*?*/ CreateMockMethod(Method m, List<TypeArgumentInstantiation> typeArgs, bool createBody, bool forBodyInheritance, bool lookasideBody);
       ConcreteSyntaxTree/*?*/ CreateFunction(string name, List<TypeArgumentInstantiation> typeArgs, List<Formal> formals, Type resultType, Bpl.IToken tok, bool isStatic, bool createBody,
         MemberDecl member, bool forBodyInheritance, bool lookasideBody);
       ConcreteSyntaxTree/*?*/ CreateGetter(string name, TopLevelDecl enclosingDecl, Type resultType, Bpl.IToken tok, bool isStatic, bool isConst, bool createBody, MemberDecl/*?*/ member, bool forBodyInheritance);  // returns null iff !createBody
@@ -1259,7 +1260,12 @@ namespace Microsoft.Dafny {
         return createBody ? block : null;
       }
 
-      public ConcreteSyntaxTree CreateMockMethod(Method m) {
+      public ConcreteSyntaxTree CreateFreshMethod(Method m) {
+        throw new NotImplementedException();
+      }
+
+      public ConcreteSyntaxTree CreateMockMethod(Method m, List<TypeArgumentInstantiation> typeArgs, bool createBody, bool forBodyInheritance,
+        bool lookasideBody) {
         throw new NotImplementedException();
       }
 
@@ -1780,10 +1786,15 @@ namespace Microsoft.Dafny {
             if (Attributes.Contains(m.Attributes, "axiom")) {
               // suppress error message
             } else if (!DafnyOptions.O.DisallowExterns && Attributes.Contains(m.Attributes, "extern")) {
-              if (Attributes.Contains(m.Attributes, "mock") && m.IsStatic &&
+              if (Attributes.Contains(m.Attributes, "fresh") && m.IsStatic &&
                   m.Outs.Count == 1 && m.Ins.Count == 0 &&
                   m.Ens.Count == 1 && m.Ens.Any(ensure => ensure.E is FreshExpr)) {
-                classWriter.CreateMockMethod(m);
+                classWriter.CreateFreshMethod(m);
+              }
+              if (Attributes.Contains(m.Attributes, "mock") && m.IsStatic &&
+                  m.Outs.Count > 0 && m.Ens.Count(ensure => ensure.E is FreshExpr) == m.Outs.Count) {
+                // TODO: one ensure can contain two fresh expressions
+                classWriter.CreateMockMethod(m, CombineAllTypeArguments(m), true, true, false);
               }
             } else {
               Error(m.tok, "Method {0} has no body", errorWr, m.FullName);
